x86/OrderedLinking.v
@@ -1,0 +1,405 @@
+(* ********************* *)
+(* Author: Yuting Wang   *)
+(* Date:   Oct 2, 2019   *)
+(* ********************* *)
+
+Require Import Coqlib Integers Values Maps AST.
+Require Import Linking Errors.
+Require Import Permutation.
+
+
+(** * Linking of Asm program such that the order of internal definitions is preserved **)
+
+
+(** Bunch of properties about Permutation and PTree *)
+Lemma NoDup_list_norepet_equiv : forall A (l: list A),
+    NoDup l <-> list_norepet l.
+Proof.
+  induction l as [|a l].
+  - split; intros. constructor. constructor.
+  - split; intros. 
+    + inv H. constructor; auto. rewrite <- IHl. auto.
+    + inv H. constructor; auto. rewrite IHl. auto.
+Qed.
+
+Lemma Permutation_pres_list_norepet: forall A (l1 l2: list A),
+  list_norepet l1 -> Permutation l1 l2 -> list_norepet l2.
+Proof.
+  intros. rewrite <- NoDup_list_norepet_equiv in *.
+  eapply Permutation_NoDup; eauto.
+Qed.
+
+Lemma Permutation_NoDup_map: forall A B (f: A -> B) (l1 l2: list A),
+    Permutation l1 l2 -> NoDup (map f l1) -> NoDup (map f l2).
+Proof.
+  intros A B f l1 l2 PERM NODUP.
+  apply Permutation_NoDup with (l:= map f l1); eauto.
+  apply Permutation_map; auto.
+Qed.
+
+Lemma Permutation_pres_ptree_get_some: forall A (l1 l2: list (ident * A)) a e,
+    list_norepet (map fst l2) ->
+    Permutation l1 l2 -> (PTree_Properties.of_list l1) ! a = Some e -> 
+    (PTree_Properties.of_list l2) ! a = Some e.
+Proof. 
+  intros A l1 l2 a e NORPT PERM GET.
+  apply PTree_Properties.of_list_norepet; auto.
+  eapply Permutation_in; eauto.
+  apply PTree_Properties.in_of_list; auto.
+Qed.
+
+Lemma Permutation_pres_ptree_get: forall A (l1 l2: list (ident * A)) a,
+    list_norepet (map fst l1) -> 
+    list_norepet (map fst l2) -> 
+    Permutation l1 l2 -> 
+    (PTree_Properties.of_list l1) ! a = (PTree_Properties.of_list l2) ! a.
+Proof. 
+  intros A l1 l2 a NORPT1 NORPT2 PERM.
+  destruct ((PTree_Properties.of_list l1) ! a) eqn:GET1.
+  - symmetry. 
+    eapply Permutation_pres_ptree_get_some; eauto.
+  - destruct ((PTree_Properties.of_list l2) ! a) eqn:GET2; auto.
+    apply Permutation_sym in PERM.
+    generalize (@Permutation_pres_ptree_get_some _ _ _ a a0 NORPT1 PERM GET2).
+    intros. congruence.
+Qed.
+
+Lemma Permutation_list_norepet_map: forall A B (f: A -> B) (l1 l2: list A),
+    Permutation l1 l2 -> list_norepet (map f l1) -> list_norepet (map f l2).
+Proof.
+  intros A B f l1 l2 PERM NORPT.
+  rewrite <- NoDup_list_norepet_equiv in *.
+  eapply Permutation_NoDup_map; eauto.
+Qed.
+
+Lemma PTree_combine_permutation: forall A B C (f: option A -> option B -> option C) l1 l1' l2 l2',
+    f None None = None ->
+    Permutation l1 l1' -> Permutation l2 l2' ->
+    list_norepet (map fst l1) -> list_norepet (map fst l2) ->
+    Permutation
+      (PTree.elements
+         (PTree.combine f (PTree_Properties.of_list l1) (PTree_Properties.of_list l2)))
+      (PTree.elements
+         (PTree.combine f (PTree_Properties.of_list l1') (PTree_Properties.of_list l2'))).
+Proof.
+  intros until l2'.
+  intros F PERM1 PERM2 NORPT1 NORPT2.
+  apply NoDup_Permutation.
+  apply NoDup_map_inv with (f:=fst); auto.
+  rewrite NoDup_list_norepet_equiv.
+  apply PTree.elements_keys_norepet.
+  apply NoDup_map_inv with (f:=fst); auto.
+  rewrite NoDup_list_norepet_equiv.
+  apply PTree.elements_keys_norepet.
+  intros (id, a).
+  split; intros IN.
+  - apply PTree.elements_complete in IN.
+    apply PTree.elements_correct.
+    rewrite PTree.gcombine in *; auto.
+    rewrite <- (Permutation_pres_ptree_get _ l1 l1'); auto.
+    rewrite <- (Permutation_pres_ptree_get _ l2 l2'); auto.
+    eapply Permutation_list_norepet_map; eauto.
+    eapply Permutation_list_norepet_map; eauto.
+  - apply PTree.elements_complete in IN.
+    apply PTree.elements_correct.
+    rewrite PTree.gcombine in *; auto.
+    rewrite (Permutation_pres_ptree_get _ l1 l1'); auto.
+    rewrite (Permutation_pres_ptree_get _ l2 l2'); auto.
+    eapply Permutation_list_norepet_map; eauto.
+    eapply Permutation_list_norepet_map; eauto.
+Qed.
+
+Fixpoint PTree_extract_elements {A:Type} (ids: list ident) (t: PTree.t A) :=
+  match ids with 
+  | nil => Some (nil, t)
+  | id :: ids' =>
+    match PTree_extract_elements ids' t with
+    | None => None
+    | Some (vals, t') => 
+      match t'!id with
+      | None => None
+      | Some val => 
+        Some ((id, val) :: vals, (PTree.remove id t'))
+      end
+    end
+  end.
+
+Lemma PTree_remove_pres_in:
+  forall (A : Type) i j (t : PTree.t A) v,
+    i <> j -> In (i, v) (PTree.elements t) ->
+    In (i, v) (PTree.elements (PTree.remove j t)).
+Proof.
+  intros A i j t v NEQ IN.
+  apply PTree.elements_correct.
+  rewrite PTree.gro; eauto.
+  apply PTree.elements_complete; auto.
+Qed.
+
+Lemma PTree_remove_pres_in':
+  forall (A : Type) i j (t : PTree.t A) v,
+    In (i, v) (PTree.elements (PTree.remove j t)) ->
+    In (i, v) (PTree.elements t).
+Proof.
+  intros A i j t v IN.
+  apply PTree.elements_correct.
+  apply PTree.elements_complete in IN.
+  destruct (ident_eq i j). subst.
+  generalize (PTree.grs j t). intros. congruence.
+  erewrite <- PTree.gro; eauto.
+Qed.
+
+Lemma PTree_remove_permutation: forall A id (t: PTree.t A) a l,
+    list_norepet (map fst ((id, a) :: l)) ->
+    t ! id = Some a ->
+    Permutation (PTree.elements (PTree.remove id t)) l ->
+    Permutation (PTree.elements t) ((id, a) :: l).
+Proof.
+  intros A id t a l NORPT GET PERM.
+  apply NoDup_Permutation.
+  apply NoDup_map_inv with (f:=fst).
+  rewrite NoDup_list_norepet_equiv.
+  apply PTree.elements_keys_norepet.
+  apply NoDup_map_inv with (f:=fst).
+  rewrite NoDup_list_norepet_equiv. auto.
+  intros (id', a').
+  split; intros IN.
+  - destruct (ident_eq id id').
+    + subst.
+      apply PTree.elements_complete in IN.
+      assert (a = a') by congruence. subst.
+      apply in_eq.
+    + apply in_cons.
+      eapply Permutation_in; eauto.      
+      apply PTree_remove_pres_in; auto.
+  - destruct (ident_eq id id').
+    + subst. inv IN. 
+      * inv H. apply PTree.elements_correct; auto.
+      * cbn in NORPT. inv NORPT.
+        apply (in_map fst) in H. cbn in H.
+        contradiction.
+    + inv IN. inv H. congruence.
+      apply PTree.elements_correct.
+      rewrite <- PTree.gro with (j := id); auto.
+      apply PTree.elements_complete.
+      apply Permutation_sym in PERM.
+      eapply Permutation_in; eauto.
+Qed.      
+
+Lemma NoDup_ptree_elements: forall A (t: PTree.t A), NoDup (PTree.elements t).
+Proof.
+  intros.
+  apply NoDup_map_inv with (f:=fst).
+  rewrite NoDup_list_norepet_equiv.
+  apply PTree.elements_keys_norepet.
+Qed.
+
+Lemma PTree_remove_in_absurd: forall A id (a:A) (t:PTree.t A),
+    ~ In (id, a) (PTree.elements (PTree.remove id t)).
+Proof.
+  intros.
+  intro IN.
+  apply PTree.elements_complete in IN.
+  generalize (PTree.grs id t). intros. congruence.
+Qed. 
+
+Lemma PTree_remove_permutation': forall A id (t: PTree.t A) a,
+    t ! id = Some a ->
+    Permutation (PTree.elements t) ((id, a) :: (PTree.elements (PTree.remove id t))).
+Proof.
+  intros.
+  apply NoDup_Permutation.
+  - apply NoDup_ptree_elements.
+  - constructor.
+    apply PTree_remove_in_absurd.
+    apply NoDup_ptree_elements.
+  - intros (id', a').
+    split; intros IN.
+    + destruct (ident_eq id id').
+      * subst.
+        apply PTree.elements_complete in IN.
+        assert (a = a') by congruence. subst.
+        apply in_eq.
+      * apply in_cons.
+        eapply Permutation_in; eauto.      
+        apply PTree_remove_pres_in; auto.
+    + inv IN. inv H0. apply PTree.elements_correct; auto.
+      eapply PTree_remove_pres_in'; eauto.
+Qed.    
+
+
+Lemma PTree_extract_elements_permutation : forall {A:Type} (ids: list ident) (t t':PTree.t A) vals,
+  PTree_extract_elements ids t = Some (vals, t') ->
+  Permutation (PTree.elements t) (vals ++ (PTree.elements t')).
+Proof.
+  induction ids as [|id ids].
+  - cbn. inversion 1. subst. inv H. auto.
+  - cbn. intros t t' vals H.
+    destr_in H. destruct p. destr_in H. inv H. cbn.
+    generalize (IHids _ _ _ Heqo). intros PERM.
+    eapply Permutation_trans; eauto.
+    assert (Permutation (PTree.elements t0) ((id, a) :: PTree.elements (PTree.remove id t0))).
+    { apply PTree_remove_permutation'; auto. }
+    eapply Permutation_trans.
+    apply Permutation_app_head. exact H.
+    apply Permutation_sym. 
+    apply Permutation_middle.
+Qed.
+
+
+
+(** The main proof begins *)
+
+Section WITHFV.
+
+Context {F V: Type}.
+Context {LF: Linker F}.
+Context {LV: Linker V}.
+Variable is_fun_internal: F -> bool.
+
+Definition is_var_internal (v: globvar V) :=
+  match classify_init (gvar_init v) with
+  | Init_definitive _ => true
+  | _ => false
+  end.
+
+Definition is_def_internal (def: option (globdef F V)) : bool :=
+  match def with
+  | None => false
+  | Some g =>
+    match g with
+    | Gvar v => is_var_internal v
+    | Gfun f => is_fun_internal f
+    end
+  end.
+
+Definition filter_internal_defs (idgs: list (ident * option (globdef F V))) :=
+  filter (fun '(id,def) => is_def_internal def) idgs.
+
+Definition collect_internal_def_ids (p: program F V) :=
+  let int_defs := filter_internal_defs (prog_defs p) in
+  map fst int_defs.
+
+
+
+Definition link_prog_ordered p1 p2 :=
+  let dm1 := prog_option_defmap p1 in
+  let dm2 := prog_option_defmap p2 in
+  if ident_eq p1.(prog_main) p2.(prog_main) 
+     && list_norepet_dec ident_eq (map fst (prog_defs p1))
+     && list_norepet_dec ident_eq (map fst (prog_defs p2)) then
+    let t := PTree.combine link_prog_merge dm1 dm2 in
+    let ids1 := collect_internal_def_ids p1 in
+    let ids2 := collect_internal_def_ids p2 in
+    match PTree_extract_elements (ids1 ++ ids2) t with
+    | None => None
+    | Some (defs, t') => 
+      Some {| prog_main := p1.(prog_main);
+              prog_public := p1.(prog_public) ++ p2.(prog_public);
+              prog_defs := PTree.elements t' ++ defs |}
+    end
+  else
+    None.
+
+End WITHFV.
+
+Definition is_fundef_internal {A:Type} (fd: fundef A) : bool :=
+  match fd with
+  | Internal _ => true
+  | External _ => false
+  end.
+
+Instance Linker_prog_ordered (F V: Type) {LV: Linker V} : Linker (program (fundef F) V) := {
+  link a b := link_prog_ordered is_fundef_internal a b;
+  linkorder a b := True;
+}.
+Proof.
+  auto.
+  auto.
+  auto.
+Defined.
+
+(** matching modulo the permutation of definitions *)
+
+Definition match_prog {F V} (p tp: program F V) :=
+  Permutation (prog_defs p) (prog_defs tp) 
+  /\ prog_main p = prog_main tp
+  /\ prog_public p = prog_public tp.
+
+Lemma transf_program_match:
+  forall F V (p: program F V), match_prog p p.
+Proof.
+  intros. red. 
+  repeat (split; auto).
+Qed.
+
+
+Lemma extract_defs_exists: 
+  forall {F V: Type} {LV:Linker V} 
+    (p1 p2: program (fundef F) V) t ids1 ids2,
+    ids1 = collect_internal_def_ids is_fundef_internal p1 ->
+    ids2 = collect_internal_def_ids is_fundef_internal p2 ->
+    t = PTree.combine link_prog_merge 
+                      (prog_option_defmap p1) 
+                      (prog_option_defmap p2) ->
+    exists defs t',
+      PTree_extract_elements (ids1 ++ ids2) t = Some (defs, t').
+Proof.
+  intros F V LV p1 p2 t ids1 ids2 IDS1 IDS2 T. subst.
+  
+
+  Lemma link_prog_merge_internal_exists: 
+    forall {F V} {LV: Linker V} 
+      (defs1: list (ident * option (globdef (fundef F) V))) ids1 t t2 id,
+      ids1 = map fst (filter_internal_defs is_fundef_internal defs1) ->
+      t = PTree.combine link_prog_merge (PTree_Properties.of_list defs1) t2 ->
+      In id ids1 -> 
+      exists def, t!id = def.
+  Admitted.
+  
+  unfold collect_internal_def_ids. 
+  unfold prog_option_defmap.
+  
+Admitted.
+
+
+
+(** Commutativity between permutation and linking *)
+Instance TransfPermuteLink {F V} {LV: Linker V}
+  : @TransfLink _ _ (Linker_prog (fundef F) V) (Linker_prog_ordered F V) match_prog.
+Proof.
+  Local Transparent Linker_prog.
+  red. unfold match_prog. cbn. 
+  intros until p.
+  intros LINK (PERM1 & MAINEQ1 & PUBEQ1) (PERM2 & MAINEQ2 & PUBEQ2).
+  unfold link_prog in LINK.
+  destr_in LINK. inv LINK. cbn.
+  repeat (rewrite andb_true_iff in Heqb). 
+  destruct Heqb as (((MAINEQ & NORPT1) & NORPT2) & CHECK).
+  destruct ident_eq; try discriminate.
+  destruct list_norepet_dec; try discriminate.
+  destruct list_norepet_dec; try discriminate.
+  unfold link_prog_ordered.
+  assert (prog_main tp1 = prog_main tp2) as MAINEQ3 by congruence.
+  rewrite MAINEQ3.
+  destruct ident_eq; try congruence. cbn.
+  assert (list_norepet (map fst (prog_defs tp1))) as NORPT3.
+  { eapply Permutation_list_norepet_map; eauto. }
+  destruct list_norepet_dec; try contradiction. cbn.
+  assert (list_norepet (map fst (prog_defs tp2))) as NORPT4.
+  { eapply Permutation_list_norepet_map; eauto. }
+  destruct list_norepet_dec; try contradiction. cbn.  
+  edestruct (@extract_defs_exists F V _ tp1 tp2) as (defs1 & t1 & EXTR); eauto.
+  rewrite EXTR. 
+  eexists; split; eauto.
+  cbn.
+  repeat (split; auto).
+  generalize (PTree_extract_elements_permutation _ _ _ _ EXTR).
+  intros PERM3. 
+  apply Permutation_trans with (defs1 ++ PTree.elements t1).
+  eapply Permutation_trans; [| exact PERM3].
+  unfold prog_option_defmap.
+  eapply PTree_combine_permutation; eauto.
+  apply Permutation_app_comm.
+  congruence.
+  congruence.
+Qed.
